starts compiling but still fake

backend/CSE3analysisaux.ml
@@ -1,0 +1,36 @@
+open CSE3analysis
+open Maps
+open HashedSet
+open Camlcoq
+
+let flatten_eq eq =
+  ((P.to_int eq.eq_lhs), eq.eq_op, List.map P.to_int eq.eq_args);;
+
+let preanalysis (f : RTL.coq_function) =
+  let cur_eq_id = ref 0
+  and cur_catalog = ref PTree.empty
+  and eq_table = Hashtbl.create 100
+  and rhs_table = Hashtbl.create 100
+  and cur_kill_reg = ref (PMap.init PSet.empty)
+  and cur_kill_mem = ref PSet.empty
+  and cur_moves = ref (PMap.init PSet.empty) in
+  let eq_find_oracle node eq =
+    Hashtbl.find_opt eq_table (flatten_eq eq)
+  and rhs_find_oracle node sop args =
+    match Hashtbl.find_opt rhs_table (sop, List.map P.to_int args) with
+    | None -> PSet.empty
+    | Some s -> s in
+  let mutating_eq_find_oracle node eq =
+    incr cur_eq_id; None in (* FIXME *)
+  ignore 
+    (internal_analysis
+      { eq_catalog     = (fun eq_id -> PTree.get eq_id !cur_catalog);
+        eq_find_oracle = mutating_eq_find_oracle;
+        eq_rhs_oracle  = rhs_find_oracle ;
+        eq_kill_reg    = (fun reg -> PMap.get reg !cur_kill_reg);
+        eq_kill_mem    = (fun () -> !cur_kill_mem);
+        eq_moves       = (fun reg -> PMap.get reg !cur_moves)
+      } f);
+  { hint_eq_catalog    = !cur_catalog;
+    hint_eq_find_oracle= eq_find_oracle;
+    hint_eq_rhs_oracle = rhs_find_oracle };;
