backend/CSE3proof.v
@@ -1,0 +1,138 @@
+(*
+Replace available expressions by the register containing their value.
+
+Proofs.
+
+David Monniaux, CNRS, VERIMAG
+ *)
+
+Require Import Coqlib Maps Errors Integers Floats Lattice Kildall.
+Require Import AST Linking.
+Require Import Memory Registers Op RTL Maps.
+
+Require Import Globalenvs Values.
+Require Import Linking Values Memory Globalenvs Events Smallstep.
+Require Import Registers Op RTL.
+Require Import CSE3 CSE3analysis CSE3analysisproof.
+
+
+Section SOUNDNESS.
+  Variable F V : Type.
+  Variable genv: Genv.t F V.
+  Variable sp : val.
+End SOUNDNESS.
+
+
+Definition match_prog (p tp: RTL.program) :=
+  match_program (fun cu f tf => tf = transf_fundef f) eq p tp.
+
+Lemma transf_program_match:
+  forall p, match_prog p (transf_program p).
+Proof.
+  intros. apply match_transform_program; auto.
+Qed.
+
+Section PRESERVATION.
+
+Variables prog tprog: program.
+Hypothesis TRANSL: match_prog prog tprog.
+Let ge := Genv.globalenv prog.
+Let tge := Genv.globalenv tprog.
+
+Lemma functions_translated:
+  forall v f,
+  Genv.find_funct ge v = Some f ->
+  Genv.find_funct tge v = Some (transf_fundef f).
+Proof (Genv.find_funct_transf TRANSL).
+
+Lemma function_ptr_translated:
+  forall v f,
+  Genv.find_funct_ptr ge v = Some f ->
+  Genv.find_funct_ptr tge v = Some (transf_fundef f).
+Proof (Genv.find_funct_ptr_transf TRANSL).
+
+Lemma symbols_preserved:
+  forall id,
+  Genv.find_symbol tge id = Genv.find_symbol ge id.
+Proof (Genv.find_symbol_transf TRANSL).
+
+Lemma senv_preserved:
+  Senv.equiv ge tge.
+Proof (Genv.senv_transf TRANSL).
+
+Lemma sig_preserved:
+  forall f, funsig (transf_fundef f) = funsig f.
+Proof.
+  destruct f; trivial.
+Qed.
+
+Lemma find_function_translated:
+  forall ros rs fd,
+  find_function ge ros rs = Some fd ->
+  find_function tge ros rs = Some (transf_fundef fd).
+Proof.
+  unfold find_function; intros. destruct ros as [r|id].
+  eapply functions_translated; eauto.
+  rewrite symbols_preserved. destruct (Genv.find_symbol ge id); try congruence.
+  eapply function_ptr_translated; eauto.
+Qed.
+
+Inductive match_frames: RTL.stackframe -> RTL.stackframe -> Prop :=
+| match_frames_intro: forall res f sp pc rs,
+    (* (forall m : mem,
+     forall vres, (fmap_sem' sp m (forward_map f) pc rs # res <- vres)) -> *)
+    match_frames (Stackframe res f sp pc rs)
+                 (Stackframe res (transf_function f) sp pc rs).
+
+Inductive match_states: RTL.state -> RTL.state -> Prop :=
+  | match_regular_states: forall stk f sp pc rs m stk'
+                                 (STACKS: list_forall2 match_frames stk stk'),
+      (* (fmap_sem' sp m (forward_map f) pc rs) -> *)
+      match_states (State stk f sp pc rs m)
+                   (State stk' (transf_function f) sp pc rs m)
+  | match_callstates: forall stk f args m stk'
+        (STACKS: list_forall2 match_frames stk stk'),
+      match_states (Callstate stk f args m)
+                   (Callstate stk' (transf_fundef f) args m)
+  | match_returnstates: forall stk v m stk'
+        (STACKS: list_forall2 match_frames stk stk'),
+      match_states (Returnstate stk v m)
+                   (Returnstate stk' v m).
+  
+
+Lemma step_simulation:
+  forall S1 t S2, RTL.step ge S1 t S2 ->
+  forall S1', match_states S1 S1' ->
+              exists S2', RTL.step tge S1' t S2' /\ match_states S2 S2'.
+Proof.
+Admitted.
+Lemma transf_initial_states:
+  forall S1, RTL.initial_state prog S1 ->
+  exists S2, RTL.initial_state tprog S2 /\ match_states S1 S2.
+Proof.
+  intros. inv H. econstructor; split.
+  econstructor.
+    eapply (Genv.init_mem_transf TRANSL); eauto.
+    rewrite symbols_preserved. rewrite (match_program_main TRANSL). eauto.
+    eapply function_ptr_translated; eauto.
+    rewrite <- H3; apply sig_preserved.
+  constructor. constructor.
+Qed.
+
+Lemma transf_final_states:
+  forall S1 S2 r, match_states S1 S2 -> RTL.final_state S1 r -> RTL.final_state S2 r.
+Proof.
+  intros. inv H0. inv H. inv STACKS. constructor.
+Qed.
+
+Theorem transf_program_correct:
+  forward_simulation (RTL.semantics prog) (RTL.semantics tprog).
+Proof.
+  eapply forward_simulation_step.
+  apply senv_preserved.
+  eexact transf_initial_states.
+  eexact transf_final_states.
+  exact step_simulation.
+Qed.
+
+End PRESERVATION.
