Makefile
@@ -89,7 +89,7 @@ BACKEND=\
   CSEdomain.v CombineOp.v CSE.v CombineOpproof.v CSEproof.v \
   CSE2deps.v CSE2depsproof.v \
   CSE2.v CSE2proof.v \
-  CSE3analysis.v \
+  CSE3analysis.v CSE3analysisproof.v CSE3.v CSE3proof.v \
   NeedDomain.v NeedOp.v Deadcode.v Deadcodeproof.v \
   Unusedglob.v Unusedglobproof.v \
   Machregs.v Locations.v Conventions1.v Conventions.v LTL.v \
